fstar/api/MLS.API.fst
@@ -1,0 +1,256 @@
+module MLS.API
+
+open MLS.TreeSync.Invariants.AuthService
+open MLS.NetworkTypes
+open MLS.TreeSync.NetworkTypes
+open MLS.TreeKEM.NetworkTypes
+open MLS.TreeDEM.NetworkTypes
+
+val no_asp:
+  #bytes:Type0 -> {|bytes_like bytes|} ->
+  as_parameters bytes
+let no_asp #bytes #bl = {
+  token_t = unit;
+  credential_ok = (fun _ _ -> True);
+  valid_successor = (fun _ _ -> True);
+}
+
+instance high_entropy (bytes:Type0) (entropy_t:Type) {|entropy bytes entropy_t|}: MLS.API.High.entropy bytes entropy_t = {
+  rel = (fun _ _ -> True);
+  rel_refl = (fun _ -> ());
+  rel_trans = (fun _ _ _ -> ());
+  extract_entropy_ = (fun n e -> extract_entropy n e);
+}
+
+// workaround for FStarLang/FStar#3311
+// to avoid having to `let open MLS.API.High`
+// and then having to reference our types / functions with MLS.API._
+val (let*?):
+  #bytes:Type0 -> #entropy_t:Type -> {|entropy bytes entropy_t|} ->
+  #a:Type -> #b:Type ->
+  MLS.API.High.prob (result a) -> (a -> MLS.API.High.prob (result b)) -> MLS.API.High.prob (result b)
+let (let*?) #bytes #entropy_t #entropy_tc #a #b x f =
+  let open MLS.API.High in
+  let*? x0 = x in
+  f x0
+
+type mls_group bytes #cb = MLS.API.High.mls_group bytes no_asp
+type unvalidated_proposal bytes #cb = MLS.API.High.unvalidated_proposal bytes
+type validated_proposal bytes #cb = MLS.API.High.validated_proposal bytes no_asp
+type unvalidated_commit bytes #cb = MLS.API.High.unvalidated_commit bytes
+type validated_commit bytes #cb = MLS.API.High.validated_commit bytes no_asp
+type credential bytes #cb = MLS.API.High.credential bytes
+type credential_pair bytes #cb = MLS.API.High.credential_pair bytes no_asp
+type signature_keypair bytes #cb = MLS.API.High.signature_keypair bytes
+
+let generate_signature_keypair #bytes #cb #entropy_t #entropy_tc =
+  MLS.API.High.generate_signature_keypair
+
+let get_signature_public_key #bytes #cb sig_keypair =
+  MLS.API.High.get_signature_public_key sig_keypair
+
+let mk_basic_credential #bytes #cb sig_keypair identity =
+  let? identity = mk_mls_bytes identity "mk_basic_credential" "identity" in
+  let cred = MLS.NetworkTypes.C_basic identity in
+  return (MLS.API.High.mk_credential sig_keypair cred ())
+
+let mk_x509_credential #bytes #cb sig_keypair x509_chain =
+  let? x509_chain = mapM (fun x -> mk_mls_bytes x "mk_x509_credential" "certificate") x509_chain in
+  let? x509_chain = mk_mls_list x509_chain "mk_basic_credential" "x509_chain" in
+  let cred = MLS.NetworkTypes.C_x509 x509_chain in
+  return (MLS.API.High.mk_credential sig_keypair cred ())
+
+let get_public_credential #bytes #cb cred_pair =
+  MLS.API.High.get_public_credential cred_pair
+
+let create_key_package #bytes #cb #entropy #entropy_t cred_pair =
+  let*? res = MLS.API.High.create_key_package cred_pair in
+  MLS.API.High.return_prob (return ({
+    key_package = serialize _ res.key_package;
+    keystore_key = res.keystore_key;
+    keystore_value = serialize _ res.keystore_value;
+  } <: create_key_package_result bytes))
+
+let create_group #bytes #cb #entropy_t #entropy_tc cred_pair =
+  MLS.API.High.create_group cred_pair
+
+let start_join_group_output bytes #cb = MLS.API.High.start_join_group_output bytes
+
+val lift_key_lookup:
+  #bytes:Type0 -> {|crypto_bytes bytes|} ->
+  key_lookup bytes ->
+  MLS.API.High.key_lookup bytes
+let lift_key_lookup #bytes #cb key_lookup b =
+  match key_lookup b with
+  | None -> None
+  | Some k -> parse _ k
+
+let start_join_group #bytes #cb welcome_bytes key_lookup =
+  let? welcome = from_option "start_join_group: malformed welcome" (parse _ welcome_bytes) in
+  MLS.API.High.start_join_group welcome (lift_key_lookup key_lookup)
+
+let continue_join_group_output bytes #cb = MLS.API.High.continue_join_group_output bytes
+
+let continue_join_group #bytes #cb step_before opt_ratchet_tree_bytes =
+  let? opt_ratchet_tree =
+    match opt_ratchet_tree_bytes with
+    | None -> return None
+    | Some ratchet_tree_bytes ->
+      let? ratchet_tree = from_option "continue_join_group: malformed ratchet tree" (parse _ ratchet_tree_bytes) in
+      return (Some ratchet_tree)
+  in
+  MLS.API.High.continue_join_group step_before opt_ratchet_tree
+
+val create_tokens:
+  #bytes:Type0 -> {|bytes_like bytes|} ->
+  leaves:list (option (leaf_node_nt bytes tkt)) ->
+  tokens:list (option ((no_asp #bytes).token_t)){List.Tot.length tokens == List.Tot.length leaves}
+let rec create_tokens #bytes #bl leaves =
+  match leaves with
+  | [] -> []
+  | h::t ->
+    (
+      match h with
+      | Some _ -> Some ()
+      | None -> None
+    )::(create_tokens t)
+
+let finalize_join_group #bytes #cb step_before =
+  MLS.API.High.finalize_join_group step_before (create_tokens (MLS.Tree.get_leaf_list step_before.treesync))
+
+let export_secret #bytes #cb st label context len =
+  MLS.API.High.export_secret st label context len
+
+let epoch_authenticator #bytes #cb st =
+  return (MLS.API.High.epoch_authenticator st)
+
+let epoch #bytes #cb st =
+  return (MLS.API.High.epoch st)
+
+let get_new_credentials #bytes #cb commit =
+  magic()
+
+let get_new_credential #bytes #cb proposal =
+  magic()
+
+let process_message #bytes #cb st msg_bytes =
+  let? msg = from_option "process_message: malformed message" (parse _ msg_bytes) in
+  let? (res, st) = MLS.API.High.process_message st msg in
+  let translated_res_content =
+    match res.content with
+    | MLS.API.High.ApplicationMessage msg -> ApplicationMessage msg
+    | MLS.API.High.Proposal proposal -> Proposal proposal
+    | MLS.API.High.Commit commit -> Commit commit
+  in
+  let translated_res = {
+    group_id = res.group_id;
+    epoch = res.epoch;
+    sender = res.sender;
+    authenticated_data = res.authenticated_data;
+    content = translated_res_content;
+  } in
+  return (translated_res, st)
+
+val mk_proposal_token_for:
+  #bytes:Type0 -> {|bytes_like bytes|} ->
+  proposal:proposal_nt bytes ->
+  MLS.API.High.proposal_token_for no_asp proposal
+let mk_proposal_token_for #bytes #bl proposal = ()
+
+val mk_proposal_tokens_for:
+  #bytes:Type0 -> {|bytes_like bytes|} ->
+  proposals: list (proposal_nt bytes) ->
+  MLS.API.High.list_to_type (List.Tot.map (MLS.API.High.proposal_token_for no_asp) proposals)
+let rec mk_proposal_tokens_for #bytes #bl l =
+  match l with
+  | [] -> ()
+  | h::t ->
+    (mk_proposal_token_for h, mk_proposal_tokens_for t)
+
+val mk_update_path_token:
+  #bytes:Type0 -> {|bytes_like bytes|} ->
+  opt_path:option (update_path_nt bytes) ->
+  MLS.API.High.update_path_token no_asp opt_path
+let mk_update_path_token #bytes #bl opt_path = ()
+
+val mk_commit_tokens_for:
+  #bytes:Type0 -> {|bytes_like bytes|} ->
+  commit:commit_nt bytes ->
+  MLS.API.High.commit_tokens_for no_asp commit
+let mk_commit_tokens_for #bytes #bl commit =
+  (mk_update_path_token commit.path, mk_proposal_tokens_for (MLS.API.High.filter_and_map MLS.API.High._get_proposal commit.proposals))
+
+let i_hereby_declare_that_i_have_checked_the_new_credentials_and_validate_the_commit #bytes #cb commit =
+  {
+    commit;
+    tokens = mk_commit_tokens_for commit.commit_msg.content.content.content;
+  }
+
+let merge_commit #bytes #cb st commit =
+  MLS.API.High.merge_commit st commit
+
+let i_hereby_declare_that_i_have_checked_the_new_credentials_and_validate_the_proposal #bytes #cb proposal = {
+  proposal;
+  token = mk_proposal_token_for proposal.proposal_msg.content.content.content;
+}
+
+let queue_new_proposal #bytes #cb st proposal =
+  MLS.API.High.queue_new_proposal st proposal
+
+val translate_framing_params:
+  #bytes:Type0 -> {|bytes_like bytes|} ->
+  framing_params bytes ->
+  MLS.API.High.framing_params bytes
+let translate_framing_params #bytes #bl fparams =
+  let { encrypt; padding_size; authenticated_data; } = fparams in
+  { encrypt; padding_size; authenticated_data; }
+
+let send_application_message #bytes #cb #entropy_t #entropy_tc st fparams message =
+  let*? (msg, st) = MLS.API.High.send_application_message st (translate_framing_params fparams) message in
+  MLS.API.High.return_prob (return (serialize _ msg, st))
+
+let propose_add_member #bytes #cb #entropy_t #entropy_tc st fparams key_package_bytes =
+  let*? key_package = MLS.API.High.return_prob (from_option "propose_add_member: malformed key package" (parse _ key_package_bytes)) in
+  let*? (msg, st) = MLS.API.High.propose_add_member st (translate_framing_params fparams) key_package in
+  MLS.API.High.return_prob (return (serialize _ msg, st))
+
+let propose_remove_member #bytes #cb #entropy_t #entropy_tc st fparams cred_to_remove =
+  let*? (msg, st) = MLS.API.High.propose_remove_member st (translate_framing_params fparams) cred_to_remove.cred in
+  MLS.API.High.return_prob (return (serialize _ msg, st))
+
+let propose_remove_myself #bytes #cb #entropy_t #entropy_tc st fparams =
+  let*? (msg, st) = MLS.API.High.propose_remove_myself st (translate_framing_params fparams) in
+  MLS.API.High.return_prob (return (serialize _ msg, st))
+
+val translate_leaf_node_params:
+  #bytes:Type0 -> {|bytes_like bytes|} ->
+  leaf_node_params bytes ->
+  MLS.API.High.leaf_node_params bytes no_asp
+let translate_leaf_node_params #bytes #bl lnparams =
+  let { nothing_yet } = lnparams in
+  { nothing_yet }
+
+val translate_commit_params:
+  #bytes:Type0 -> {|bytes_like bytes|} ->
+  commit_params bytes ->
+  MLS.API.High.commit_params bytes no_asp
+let translate_commit_params #bytes #bl cparams =
+  let { proposals; inline_tree; force_update; leaf_node_params; } = cparams in
+  {
+    proposals = List.Tot.map (fun proposal -> { proposal; token = mk_proposal_token_for proposal; } <: MLS.API.High.bare_proposal_and_token bytes no_asp) proposals;
+    inline_tree;
+    force_update;
+    leaf_node_params = translate_leaf_node_params leaf_node_params;
+  }
+
+let create_commit #bytes #cb st fparams cparams =
+  let*? (commit, opt_welcome, group_info, st) = MLS.API.High.create_commit st (translate_framing_params fparams) (translate_commit_params cparams) in
+  MLS.API.High.return_prob (return ({
+    commit = serialize _ commit;
+    welcome = (
+      match opt_welcome with
+      | None -> None
+      | Some welcome -> Some (serialize _ welcome)
+    );
+    group_info = serialize _ group_info;
+  }, st))
